ulib/FStar.Reflection.Arith.fst
@@ -23,12 +23,13 @@ type expr =
     | Plus  : expr -> expr -> expr
     | Mult  : expr -> expr -> expr
     | Minus : expr -> expr -> expr
-    | Land    : expr -> expr -> expr
-    | Lxor    : expr -> expr -> expr
-    | Shl     : expr -> expr -> expr
-    | Shr     : expr -> expr -> expr
-    | Neg     : expr -> expr
-    | NatToBv : expr -> expr
+    | Land  : expr -> expr -> expr -> expr
+    | Lxor  : expr -> expr -> expr -> expr
+    | Lor   : expr -> expr -> expr -> expr
+    | Shl   : expr -> expr -> expr -> expr
+    | Shr   : expr -> expr -> expr -> expr
+    | Neg   : expr -> expr
+    | NatToBv : expr -> expr -> expr
     // | Div   : expr -> expr -> expr // Add this one?
 
 noeq
@@ -69,6 +70,14 @@ let liftM2 f x y =
     yy <-- y;
     return (f xx yy)
 
+val liftM3 : ('a -> 'b -> 'c -> 'd) -> (tm 'a -> tm 'b -> tm 'c -> tm 'd)
+let liftM3 f x y z =
+    xx <-- x;
+    yy <-- y;
+    zz <-- z;
+    return (f xx yy zz)
+
+
 private let rec find_idx (f : 'a -> bool) (l : list 'a) : option ((n:nat{n < List.length l}) * 'a) =
     match l with
     | [] -> None
@@ -97,6 +106,18 @@ val is_arith_expr : term -> tm expr
 let rec is_arith_expr (t:term) =
     let hd, tl = collect_app t in
     match inspect hd, tl with
+    | Tv_FVar fv, [e1; e2 ;e3] ->
+      let qn = inspect_fv fv in
+      collect_app_order t;
+      let e1' = is_arith_expr (e1 <: x:term{x << t}) in
+      let e2' = is_arith_expr (e2 <: x:term{x << t}) in
+      let e3' = is_arith_expr (e3 <: x:term{x << t}) in
+      if qn = land_qn then liftM3 Land e1' e2' e3'
+      else if qn = lxor_qn then liftM3 Lxor e1' e2' e3'
+      else if qn = lor_qn then liftM3 Lor e1' e2' e3'
+      else if qn = shiftr_qn then liftM3 Shr e1' e2' e3'
+      else if qn = shiftl_qn then liftM3 Shl e1' e2' e3'
+      else fail ("triary: " ^ fv_to_string fv)
     | Tv_FVar fv, [l; r] ->
         let qn = inspect_fv fv in
         collect_app_order t;
@@ -108,17 +129,13 @@ let rec is_arith_expr (t:term) =
         else if qn = minus_qn then liftM2 Minus ll rr
         else if qn = mult_qn  then liftM2 Mult ll rr
         else if qn = mult'_qn then liftM2 Mult ll rr
-	else if qn = land_qn then liftM2 Land ll rr
-	else if qn = lxor_qn then liftM2 Lxor ll rr
-	else if qn = shiftr_qn then liftM2 Shr ll rr
-	else if qn = shiftl_qn then liftM2 Shl ll rr
+	else if qn = nat_bv_qn then liftM2 NatToBv ll rr
         else fail ("binary: " ^ fv_to_string fv)
     | Tv_FVar fv, [a] ->
         let qn = inspect_fv fv in
         collect_app_order t;
         let aa = is_arith_expr (a <: x:term{x << t}) in
         if qn = neg_qn then liftM Neg aa
-	else if qn = nat_bv_qn then liftM NatToBv aa
         else fail ("unary: " ^ fv_to_string fv)
     | Tv_Const (C_Int i), _ ->
         return (Lit i)
