ulib/FStar.Tactics.BV.fst
@@ -7,35 +7,41 @@ open FStar.BitVector
 open FStar.UInt
 
 (* Lemmas transforming integer arithmetic to bitvector arithmetic *)
-val to_vec_land : (#n:pos) -> (#x:uint_t n) -> (#y:uint_t n) -> (#z:bv_t n) ->
+val to_vec_logand : (#n:pos) -> (#x:uint_t n) -> (#y:uint_t n) -> (#z:bv_t n) ->
 			    squash (logand_vec #n (to_vec #n x) (to_vec #n y) == z) ->
 			    Lemma (to_vec #n (logand #n x y) == z)
-let to_vec_land #n #x #y #z pf =
+let to_vec_logand #n #x #y #z pf =
   inverse_vec_lemma #n (logand_vec #n (to_vec x) (to_vec y));
   ()
   
 
-val to_vec_lxor : #n:pos -> (#x:uint_t n) -> (#y:uint_t n) -> (#z:bv_t n) ->
+val to_vec_logxor : #n:pos -> (#x:uint_t n) -> (#y:uint_t n) -> (#z:bv_t n) ->
 		     squash (logxor_vec (to_vec x) (to_vec y) == z) ->
 		     Lemma (to_vec (logxor x y) == z)
-let to_vec_lxor #n #x #y #z pf =
+let to_vec_logxor #n #x #y #z pf =
   inverse_vec_lemma #n (logxor_vec #n (to_vec x) (to_vec y));
   ()
 
-val to_vec_lor : #n:pos -> (#x:uint_t n) -> (#y:uint_t n) -> (#z:bv_t n) ->
+val to_vec_logor : #n:pos -> (#x:uint_t n) -> (#y:uint_t n) -> (#z:bv_t n) ->
 		     squash (logor_vec (to_vec x) (to_vec y) == z) ->
 		     Lemma (to_vec (logor x y) == z)
-let to_vec_lor #n #x #y #z pf =
+let to_vec_logor #n #x #y #z pf =
   inverse_vec_lemma #n (logor_vec #n (to_vec x) (to_vec y));
   ()
 
-assume val to_vec_shl : #n:pos -> (#x:uint_t n) -> (#y:uint_t n) -> (#z:bv_t n) ->
+val to_vec_shl : #n:pos -> (#x:uint_t n) -> (#y:uint_t n) -> (#z:bv_t n) ->
 			    squash (shift_left_vec (to_vec x) y == z) ->
 			    Lemma (to_vec (shift_left x y) == z)
-
-assume val to_vec_shr : #n:pos -> (#x:uint_t n) -> (#y:uint_t n) -> (#z:bv_t n) ->
+let to_vec_shl #n #x #y #z pf =
+  inverse_vec_lemma #n (shift_left_vec #n (to_vec x) y);			    
+  ()
+  
+val to_vec_shr : #n:pos -> (#x:uint_t n) -> (#y:uint_t n) -> (#z:bv_t n) ->
 			    squash (shift_right_vec (to_vec x) y == z) ->
 			    Lemma (to_vec (shift_right x y) == z)
+let to_vec_shr #n #x #y #z pf =
+  inverse_vec_lemma #n (shift_right_vec #n (to_vec x) y);
+  ()
 
 (* Congruence lemmas used to push integer to bitvector transformations through arguments of expressions *)
 val cong_logand_vec : #n:pos -> (#w:bv_t n) -> (#x:bv_t n) -> 
@@ -50,20 +56,21 @@ val cong_logxor_vec : #n:pos -> (#w:bv_t n) -> (#x:bv_t n) ->
 			       Lemma (logxor_vec w x == logxor_vec y z)
 let cong_logxor_vec #n #w #x #y #z pf1 pf2 = ()
 
-val cong_lor_vec : #n:pos -> (#w:bv_t n) -> (#x:bv_t n) -> 
+val cong_logor_vec : #n:pos -> (#w:bv_t n) -> (#x:bv_t n) -> 
 			       (#y:bv_t n) -> (#z:bv_t n) ->
 			       squash (w == y) -> squash (x == z) ->
 			       Lemma (logor_vec w x == logor_vec y z)
-let cong_lor_vec #n #w #x #y #z pf1 pf2 = ()
+let cong_logor_vec #n #w #x #y #z pf1 pf2 = ()
 
-assume val cong_shift_left_vec : #n:pos -> (#w:bv_t n) -> (#x:nat) -> 
+val cong_shift_left_vec : #n:pos -> (#w:bv_t n) -> (#x:uint_t n) -> 
 				 (#y:bv_t n) -> squash (w == y) ->
 				 Lemma (shift_left_vec w x == shift_left_vec y x)
+let cong_shift_left_vec #n #w #x #y pf = ()
 
-assume val cong_shift_right_vec : #n:pos -> (#w:bv_t n) -> (#x:nat) -> 
-				  (#y:bv_t n) -> squash (w == y) ->
-				  Lemma (shift_right_vec w x == shift_right_vec y x)
-
+val cong_shift_right_vec : #n:pos -> #w:bv_t n -> (#x:uint_t n) -> 
+			   #y:bv_t n -> squash (w == y) ->
+			   Lemma (shift_right_vec w x == shift_right_vec y x)
+let cong_shift_right_vec #n #w #x #y pf = ()
 
 (* Used to reduce the initial equation to an equation on bitvectors*)
 val eq_to_bv: #n:pos -> (#x:uint_t n) -> (#y:uint_t n) ->
@@ -85,37 +92,46 @@ let trans #n #x #y #z #w pf1 pf2 pf3 = ()
  *)
 let rec arith_expr_to_bv e : tactic unit =
     match e with
-    | NatToBv (Shl e1 _) | Shl e1 _ ->
+    | NatToBv _ (Shl _ e1 _) | Shl _ e1 _ ->
         apply_lemma (quote to_vec_shl);;
         apply_lemma (quote cong_shift_left_vec);;
         arith_expr_to_bv e1
-    | NatToBv (Shr e1 _) | Shr e1 _ ->
+    | NatToBv _ (Shr _ e1 _) | Shr _ e1 _ ->
         apply_lemma (quote to_vec_shr);;
         apply_lemma (quote cong_shift_right_vec);;
         arith_expr_to_bv e1
-    | NatToBv (Land e1 e2) | (Land e1 e2) ->
-        apply_lemma (quote to_vec_land);;
+    | NatToBv _ (Land _ e1 e2) | (Land _ e1 e2) ->
+        apply_lemma (quote to_vec_logand);;
+	dump "after to_vec_logand";;
         apply_lemma (quote cong_logand_vec);;
+	dump "after cong";;
         arith_expr_to_bv e1;;
         arith_expr_to_bv e2
-    | NatToBv (Lxor e1 e2) | (Lxor e1 e2) ->
-        apply_lemma (quote to_vec_lxor);;
+    | NatToBv _ (Lxor _ e1 e2) | (Lxor _ e1 e2) ->
+        apply_lemma (quote to_vec_logxor);;
         apply_lemma (quote cong_logxor_vec);;
         arith_expr_to_bv e1;;
         arith_expr_to_bv e2
+    | NatToBv _ (Lor _ e1 e2) | (Lor _ e1 e2) ->
+        apply_lemma (quote to_vec_logor);;
+        apply_lemma (quote cong_logor_vec);;
+        arith_expr_to_bv e1;;
+        arith_expr_to_bv e2	
     | _ ->
         trefl
 
 let arith_to_bv_tac : tactic unit =
-    norm [Simpl];;
+    // norm [Simpl];;
     g <-- cur_goal;
     let f = term_as_formula g in
     match f with
     | Comp Eq t l r ->
      begin match run_tm (is_arith_expr l) with
       | Inl s ->
+        dump "in left";;
         trefl
       | Inr e ->
+	    dump "before seq";;
             seq (arith_expr_to_bv e) trefl
 	   //  arith_expr_to_bv e
         end
@@ -130,5 +146,6 @@ let bv_tac ()  =
 	   apply_lemma (quote trans);;
 	   arith_to_bv_tac;;
 	   arith_to_bv_tac;;
+	   dump "after arith_to_bv";;
 	   smt ()
 
